su.nsk.iae.rpl/Derived_Patterns.thy
@@ -1,4 +1,4 @@
-theory Derived_Patterns imports VCProving.Basic_Patterns 
+theory Derived_Patterns imports Basic_Patterns 
 begin
 
 definition always2 where "always2 A11 A12 A2 s \<equiv> (always (\<lambda> r2 r1 . ((weak_previous (\<lambda> r4 r3 . (\<not> (A11 r3))) r2 r1) \<or> ((\<not> (A12 r1)) \<or> (A2 r2 r1)))) s)"
@@ -142,9 +142,9 @@ done
 
 
 
-lemmas always2_used_patterns = always2_def always_def weak_previous_def 
+lemmas always2_used_patterns = always2_def always_used_patterns weak_previous_def 
 
-lemmas always2_inv_used_patterns = always2_inv_def always_inv_def weak_previous_def previous_inv_def 
+lemmas always2_inv_used_patterns = always2_inv_def always_inv_used_patterns weak_previous_def previous_inv_def 
 
 lemmas always2_inv_part_used_patterns = always2_inv_part_def always2_inv_used_patterns
 
@@ -300,9 +300,9 @@ done
 
 
 
-lemmas P1_1_used_patterns = P1_1_def always_def constrained_until_def 
+lemmas P1_1_used_patterns = P1_1_def always_used_patterns constrained_until_def 
 
-lemmas P1_1_inv_used_patterns = P1_1_inv_def always_inv_def constrained_until_inv_def 
+lemmas P1_1_inv_used_patterns = P1_1_inv_def always_inv_used_patterns constrained_until_inv_def 
 
 lemmas P1_1_inv_part_used_patterns = P1_1_inv_part_def P1_1_inv_used_patterns
 
@@ -516,9 +516,9 @@ done
 
 
 
-lemmas P1_2_used_patterns = P1_2_def always_def weak_previous_def constrained_until_def 
+lemmas P1_2_used_patterns = P1_2_def always_used_patterns weak_previous_def constrained_until_def 
 
-lemmas P1_2_inv_used_patterns = P1_2_inv_def always_inv_def weak_previous_def constrained_until_inv_def previous_inv_def 
+lemmas P1_2_inv_used_patterns = P1_2_inv_def always_inv_used_patterns weak_previous_def constrained_until_inv_def previous_inv_def 
 
 lemmas P1_2_inv_part_used_patterns = P1_2_inv_part_def P1_2_inv_used_patterns
 
@@ -646,9 +646,9 @@ done
 
 
 
-lemmas P2_1_used_patterns = P2_1_def always_def constrained_always_def 
+lemmas P2_1_used_patterns = P2_1_def always_used_patterns constrained_always_def 
 
-lemmas P2_1_inv_used_patterns = P2_1_inv_def always_inv_def constrained_always_inv_def 
+lemmas P2_1_inv_used_patterns = P2_1_inv_def always_inv_used_patterns constrained_always_inv_def 
 
 lemmas P2_1_inv_part_used_patterns = P2_1_inv_part_def P2_1_inv_used_patterns
 
@@ -834,9 +834,9 @@ done
 
 
 
-lemmas P2_2_used_patterns = P2_2_def always_def weak_previous_def constrained_always_def 
+lemmas P2_2_used_patterns = P2_2_def always_used_patterns weak_previous_def constrained_always_def 
 
-lemmas P2_2_inv_used_patterns = P2_2_inv_def always_inv_def weak_previous_def constrained_always_inv_def previous_inv_def 
+lemmas P2_2_inv_used_patterns = P2_2_inv_def always_inv_used_patterns weak_previous_def constrained_always_inv_def previous_inv_def 
 
 lemmas P2_2_inv_part_used_patterns = P2_2_inv_part_def P2_2_inv_used_patterns
 
@@ -978,9 +978,9 @@ done
 
 
 
-lemmas P3_1_used_patterns = P3_1_def always_def weak_until_def 
+lemmas P3_1_used_patterns = P3_1_def always_used_patterns weak_until_def 
 
-lemmas P3_1_inv_used_patterns = P3_1_inv_def always_inv_def weak_until_inv_def 
+lemmas P3_1_inv_used_patterns = P3_1_inv_def always_inv_used_patterns weak_until_inv_def 
 
 lemmas P3_1_inv_part_used_patterns = P3_1_inv_part_def P3_1_inv_used_patterns
 
@@ -1180,9 +1180,9 @@ done
 
 
 
-lemmas P3_2_used_patterns = P3_2_def always_def weak_previous_def weak_until_def 
+lemmas P3_2_used_patterns = P3_2_def always_used_patterns weak_previous_def weak_until_def 
 
-lemmas P3_2_inv_used_patterns = P3_2_inv_def always_inv_def weak_previous_def weak_until_inv_def previous_inv_def 
+lemmas P3_2_inv_used_patterns = P3_2_inv_def always_inv_used_patterns weak_previous_def weak_until_inv_def previous_inv_def 
 
 lemmas P3_2_inv_part_used_patterns = P3_2_inv_part_def P3_2_inv_used_patterns
 
@@ -1360,9 +1360,9 @@ done
 
 
 
-lemmas P3_3_used_patterns = P3_3_def always_def weak_previous_def weak_until_def 
+lemmas P3_3_used_patterns = P3_3_def always_used_patterns weak_previous_def weak_until_def 
 
-lemmas P3_3_inv_used_patterns = P3_3_inv_def always_inv_def weak_previous_def weak_until_inv_def previous_inv_def 
+lemmas P3_3_inv_used_patterns = P3_3_inv_def always_inv_used_patterns weak_previous_def weak_until_inv_def previous_inv_def 
 
 lemmas P3_3_inv_part_used_patterns = P3_3_inv_part_def P3_3_inv_used_patterns
 
@@ -1603,9 +1603,9 @@ done
 
 
 
-lemmas P3_4_used_patterns = P3_4_def always_def weak_previous_def weak_previous_def weak_until_def 
+lemmas P3_4_used_patterns = P3_4_def always_used_patterns weak_previous_def weak_previous_def weak_until_def 
 
-lemmas P3_4_inv_used_patterns = P3_4_inv_def always_inv_def weak_previous_def weak_previous_def weak_until_inv_def previous_inv_def weak_previous_def previous_inv_def 
+lemmas P3_4_inv_used_patterns = P3_4_inv_def always_inv_used_patterns weak_previous_def weak_previous_def weak_until_inv_def previous_inv_def weak_previous_def previous_inv_def 
 
 lemmas P3_4_inv_part_used_patterns = P3_4_inv_part_def P3_4_inv_used_patterns
 
@@ -1761,9 +1761,9 @@ done
 
 
 
-lemmas P4_1_used_patterns = P4_1_def always_def constrained_weak_until_def 
+lemmas P4_1_used_patterns = P4_1_def always_used_patterns constrained_weak_until_def 
 
-lemmas P4_1_inv_used_patterns = P4_1_inv_def always_inv_def constrained_weak_until_inv_def 
+lemmas P4_1_inv_used_patterns = P4_1_inv_def always_inv_used_patterns constrained_weak_until_inv_def 
 
 lemmas P4_1_inv_part_used_patterns = P4_1_inv_part_def P4_1_inv_used_patterns
 
@@ -1977,27 +1977,27 @@ done
 
 
 
-lemmas P4_2_used_patterns = P4_2_def always_def weak_previous_def constrained_weak_until_def 
+lemmas P4_2_used_patterns = P4_2_def always_used_patterns weak_previous_def constrained_weak_until_def 
 
-lemmas P4_2_inv_used_patterns = P4_2_inv_def always_inv_def weak_previous_def constrained_weak_until_inv_def previous_inv_def 
+lemmas P4_2_inv_used_patterns = P4_2_inv_def always_inv_used_patterns weak_previous_def constrained_weak_until_inv_def previous_inv_def 
 
 lemmas P4_2_inv_part_used_patterns = P4_2_inv_part_def P4_2_inv_used_patterns
 
 lemmas P4_2_part_used_patterns = P4_2_part_def P4_2_used_patterns
 
-definition P4_3 where "P4_3 t A11 A12 A21 A22 A3 s \<equiv> (always (\<lambda> r2 r1 . ((weak_previous (\<lambda> r4 r3 . (\<not> (A11 r3))) r2 r1) \<or> ((\<not> (A12 r1)) \<or> (constrained_weak_until t (\<lambda> r4 r3 . ((previous A21 r4 r3) \<and> (A22 r4 r3))) A3 r2 r1)))) s)"
+definition P4_3 where "P4_3 t A11 A12 A2 A31 A32 s \<equiv> (always (\<lambda> r2 r1 . ((weak_previous (\<lambda> r4 r3 . (\<not> (A11 r3))) r2 r1) \<or> ((\<not> (A12 r1)) \<or> (constrained_weak_until t A2 (\<lambda> r4 r3 . ((previous A31 r4 r3) \<and> (A32 r4 r3))) r2 r1)))) s)"
 
-definition P4_3_part where "P4_3_part t A11 A12 A21 A22 A3 s \<equiv> (P4_3 t A11 A12 (\<lambda> s s1 . (A21 s1)) (\<lambda> s s1 . (A22 s1)) (\<lambda> s s1 . (A3 s1)) s)"
+definition P4_3_part where "P4_3_part t A11 A12 A2 A31 A32 s \<equiv> (P4_3 t A11 A12 (\<lambda> s s1 . (A2 s1)) (\<lambda> s s1 . (A31 s1)) (\<lambda> s s1 . (A32 s1)) s)"
 
-definition P4_3_inv where "P4_3_inv t b_0 b_1 t1_0 A11 A12 A21_1 A22_1 A3_1 s \<equiv> (((always_inv (\<lambda> r2 r1 . ((weak_previous (\<lambda> r4 r3 . (\<not> (A11 r3))) r2 r1) \<or> ((\<not> (A12 r1)) \<or> (constrained_weak_until_inv t t1_0 (\<lambda> r4 r3 . ((previous A21_1 r4 r3) \<and> (A22_1 r4 r3))) A3_1 r2 r1)))) s) \<and> (previous_inv b_0 (\<lambda> r4 r3 . (\<not> (A11 r3))) s)) \<and> (previous_inv b_1 A21_1 s))"
+definition P4_3_inv where "P4_3_inv t b_0 b_1 t1_0 A11 A12 A2_1 A31_1 A32_1 s \<equiv> (((always_inv (\<lambda> r2 r1 . ((weak_previous (\<lambda> r4 r3 . (\<not> (A11 r3))) r2 r1) \<or> ((\<not> (A12 r1)) \<or> (constrained_weak_until_inv t t1_0 A2_1 (\<lambda> r4 r3 . ((previous A31_1 r4 r3) \<and> (A32_1 r4 r3))) r2 r1)))) s) \<and> (previous_inv b_0 (\<lambda> r4 r3 . (\<not> (A11 r3))) s)) \<and> (previous_inv b_1 A31_1 s))"
 
-definition P4_3_inv_part where "P4_3_inv_part t b_0 b_1 t1_0 A11 A12 A21 A22 A3 s \<equiv> (P4_3_inv t b_0 b_1 t1_0 A11 A12 (\<lambda> s s1 . (A21 s1)) (\<lambda> s s1 . (A22 s1)) (\<lambda> s s1 . (A3 s1)) s)"
+definition P4_3_inv_part where "P4_3_inv_part t b_0 b_1 t1_0 A11 A12 A2 A31 A32 s \<equiv> (P4_3_inv t b_0 b_1 t1_0 A11 A12 (\<lambda> s s1 . (A2 s1)) (\<lambda> s s1 . (A31 s1)) (\<lambda> s s1 . (A32 s1)) s)"
 
 lemma P4_3_inv_saving_gen: "
-P4_3_inv t b_0 b_1 t1_0 A11 A12 A21_1 A22_1 A3_1 s0 \<Longrightarrow>
+P4_3_inv t b_0 b_1 t1_0 A11 A12 A2_1 A31_1 A32_1 s0 \<Longrightarrow>
 consecutive s0 s \<Longrightarrow>
-((((True \<and> (True \<and> (((always_imp s0 (A21_1 s0) (A21_1 s)) \<and> (always_imp s0 (\<lambda> r3 . (A22_1 s0 r3)) (\<lambda> r3 . (A22_1 s r3)))) \<and> ((always_imp s0 (A3_1 s0) (A3_1 s)) \<and> ((((t1_0 s0) < t) \<and> (((A3_1 s s) \<and> ((t1_0 s) <= (t + 1))) \<or> (((t1_0 s) <= ((t1_0 s0) + 1)) \<and> (((b_1 s0) \<and> (always_imp s0 (A21_1 s0) (A21_1 s))) \<and> (A22_1 s s))))) \<or> (((t1_0 s0) >= t) \<and> ((t1_0 s) <= ((t1_0 s0) + 1)))))))) \<and> (((b_0 s0) \<and> True) \<or> ((\<not> (A12 s)) \<or> ((A3_1 s s) \<or> (((t1_0 s) = 0) \<and> (((b_1 s0) \<and> (always_imp s0 (A21_1 s0) (A21_1 s))) \<and> (A22_1 s s))))))) \<and> ((b_0 s) --> (\<not> (A11 s)))) \<and> ((b_1 s) --> (A21_1 s s))) \<Longrightarrow>
-P4_3_inv t b_0 b_1 t1_0 A11 A12 A21_1 A22_1 A3_1 s"
+((((True \<and> (True \<and> ((always_imp s0 (A2_1 s0) (A2_1 s)) \<and> (((always_imp s0 (A31_1 s0) (A31_1 s)) \<and> (always_imp s0 (\<lambda> r3 . (A32_1 s0 r3)) (\<lambda> r3 . (A32_1 s r3)))) \<and> ((((t1_0 s0) < t) \<and> (((((b_1 s0) \<and> (always_imp s0 (A31_1 s0) (A31_1 s))) \<and> (A32_1 s s)) \<and> ((t1_0 s) <= (t + 1))) \<or> (((t1_0 s) <= ((t1_0 s0) + 1)) \<and> (A2_1 s s)))) \<or> (((t1_0 s0) >= t) \<and> ((t1_0 s) <= ((t1_0 s0) + 1)))))))) \<and> (((b_0 s0) \<and> True) \<or> ((\<not> (A12 s)) \<or> ((((b_1 s0) \<and> (always_imp s0 (A31_1 s0) (A31_1 s))) \<and> (A32_1 s s)) \<or> (((t1_0 s) = 0) \<and> (A2_1 s s)))))) \<and> ((b_0 s) --> (\<not> (A11 s)))) \<and> ((b_1 s) --> (A31_1 s s))) \<Longrightarrow>
+P4_3_inv t b_0 b_1 t1_0 A11 A12 A2_1 A31_1 A32_1 s"
 
 unfolding P4_3_inv_def
 apply(erule conjE)
@@ -2040,25 +2040,25 @@ apply(erule always_rule)
               subgoal premises prems6
               apply(rule conjI)
               apply(insert prems6(1,2))[1]
-                apply(rule always_conj_rule)
-                apply simp
-                  apply(erule conjE)
-                  subgoal premises prems7
-                  apply(rule conjI)
-                  apply(insert prems7(1,2))[1]
-                    apply(rule previous_LS4)
-                    apply simp
-                      apply assumption
-                  apply(insert prems7(1,3))
-                    apply assumption
-                  done
+                apply assumption
               apply(insert prems6(1,3))
                 apply(erule conjE)
-                subgoal premises prems8
+                subgoal premises prems7
                 apply(rule conjI)
-                apply(insert prems8(1,2))[1]
-                  apply assumption
-                apply(insert prems8(1,3))
+                apply(insert prems7(1,2))[1]
+                  apply(rule always_conj_rule)
+                  apply simp
+                    apply(erule conjE)
+                    subgoal premises prems8
+                    apply(rule conjI)
+                    apply(insert prems8(1,2))[1]
+                      apply(rule previous_LS4)
+                      apply simp
+                        apply assumption
+                    apply(insert prems8(1,3))
+                      apply assumption
+                    done
+                apply(insert prems7(1,3))
                   apply(erule disjE)
                   apply(rule disjI1)
                     apply(erule conjE)
@@ -2073,34 +2073,34 @@ apply(erule always_rule)
                         subgoal premises prems10
                         apply(rule conjI)
                         apply(insert prems10(1,2))[1]
-                          apply assumption
+                          apply(erule conjE)
+                          subgoal premises prems11
+                          apply(rule conjI)
+                          apply(insert prems11(1,2))[1]
+                            apply(rule previous_one_point[OF prems1(3)])
+                            apply simp
+                              apply(erule conjE)
+                              subgoal premises prems12
+                              apply(rule conjI)
+                              apply(insert prems12(1,2))[1]
+                                apply assumption
+                              apply(insert prems12(1,3))
+                                apply assumption
+                              done
+                          apply(insert prems11(1,3))
+                            apply assumption
+                          done
                         apply(insert prems10(1,3))
                           apply assumption
                         done
                       apply(rule disjI2)
                         apply(erule conjE)
-                        subgoal premises prems11
+                        subgoal premises prems13
                         apply(rule conjI)
-                        apply(insert prems11(1,2))[1]
+                        apply(insert prems13(1,2))[1]
                           apply assumption
-                        apply(insert prems11(1,3))
-                          apply(erule conjE)
-                          subgoal premises prems12
-                          apply(rule conjI)
-                          apply(insert prems12(1,2))[1]
-                            apply(rule previous_one_point[OF prems1(3)])
-                            apply simp
-                              apply(erule conjE)
-                              subgoal premises prems13
-                              apply(rule conjI)
-                              apply(insert prems13(1,2))[1]
-                                apply assumption
-                              apply(insert prems13(1,3))
-                                apply assumption
-                              done
-                          apply(insert prems12(1,3))
-                            apply assumption
-                          done
+                        apply(insert prems13(1,3))
+                          apply assumption
                         done
                     done
                   apply(rule disjI2)
@@ -2131,31 +2131,31 @@ apply(erule always_rule)
         apply simp
           apply(erule disjE)
           apply(rule disjI1)
-            apply assumption
-          apply(rule disjI2)
             apply(erule conjE)
             subgoal premises prems15
             apply(rule conjI)
             apply(insert prems15(1,2))[1]
-              apply assumption
+              apply(rule previous_one_point[OF prems1(3)])
+              apply simp
+                apply(erule conjE)
+                subgoal premises prems16
+                apply(rule conjI)
+                apply(insert prems16(1,2))[1]
+                  apply assumption
+                apply(insert prems16(1,3))
+                  apply assumption
+                done
             apply(insert prems15(1,3))
-              apply(erule conjE)
-              subgoal premises prems16
-              apply(rule conjI)
-              apply(insert prems16(1,2))[1]
-                apply(rule previous_one_point[OF prems1(3)])
-                apply simp
-                  apply(erule conjE)
-                  subgoal premises prems17
-                  apply(rule conjI)
-                  apply(insert prems17(1,2))[1]
-                    apply assumption
-                  apply(insert prems17(1,3))
-                    apply assumption
-                  done
-              apply(insert prems16(1,3))
-                apply assumption
-              done
+              apply assumption
+            done
+          apply(rule disjI2)
+            apply(erule conjE)
+            subgoal premises prems17
+            apply(rule conjI)
+            apply(insert prems17(1,2))[1]
+              apply assumption
+            apply(insert prems17(1,3))
+              apply assumption
             done
   done
 apply(insert prems2(1,3,5))
@@ -2183,10 +2183,10 @@ done
 done
 
 lemma P4_3einv_imp_req_gen: "
-P4_3_inv t b_0 b_1 t1_0 A11 A12 A21_1 A22_1 A3_1 s0 \<Longrightarrow>
+P4_3_inv t b_0 b_1 t1_0 A11 A12 A2_1 A31_1 A32_1 s0 \<Longrightarrow>
 toEnvP s0 \<Longrightarrow>
-(True \<and> (True \<and> (((always_imp s0 (A21_1 s0) (A21 s0)) \<and> (always_imp s0 (\<lambda> r3 . (A22_1 s0 r3)) (\<lambda> r3 . (A22 s0 r3)))) \<and> (always_imp s0 (A3_1 s0) (A3 s0))))) \<Longrightarrow>
-P4_3 t A11 A12 A21 A22 A3 s0"
+(True \<and> (True \<and> ((always_imp s0 (A2_1 s0) (A2 s0)) \<and> ((always_imp s0 (A31_1 s0) (A31 s0)) \<and> (always_imp s0 (\<lambda> r3 . (A32_1 s0 r3)) (\<lambda> r3 . (A32 s0 r3))))))) \<Longrightarrow>
+P4_3 t A11 A12 A2 A31 A32 s0"
 
 unfolding P4_3_inv_def P4_3_def
 subgoal premises prems1
@@ -2221,6 +2221,8 @@ apply simp
             subgoal premises prems5
             apply(rule conjI)
             apply(insert prems5(1,2))[1]
+              apply assumption
+            apply(insert prems5(1,3))
               apply(rule always_conj_rule)
               apply simp
                 apply(erule conjE)
@@ -2233,8 +2235,6 @@ apply simp
                 apply(insert prems6(1,3))
                   apply assumption
                 done
-            apply(insert prems5(1,3))
-              apply assumption
             done
         done
     done
@@ -2243,20 +2243,20 @@ done
 done
 
 lemma P4_3_inv_saving: "
-P4_3_inv_part t b_0 b_1 t1_0 A11 A12 A21 A22 A3 s0 \<Longrightarrow>
+P4_3_inv_part t b_0 b_1 t1_0 A11 A12 A2 A31 A32 s0 \<Longrightarrow>
 consecutive s0 s \<Longrightarrow>
-(((((((t1_0 s0) < t) \<and> (((A3 s) \<and> ((t1_0 s) <= (t + 1))) \<or> (((t1_0 s) <= ((t1_0 s0) + 1)) \<and> ((b_1 s0) \<and> (A22 s))))) \<or> (((t1_0 s0) >= t) \<and> ((t1_0 s) <= ((t1_0 s0) + 1)))) \<and> ((b_0 s0) \<or> ((\<not> (A12 s)) \<or> ((A3 s) \<or> (((t1_0 s) = 0) \<and> ((b_1 s0) \<and> (A22 s))))))) \<and> ((b_0 s) --> (\<not> (A11 s)))) \<and> ((b_1 s) --> (A21 s))) \<Longrightarrow>
-P4_3_inv_part t b_0 b_1 t1_0 A11 A12 A21 A22 A3 s"
+(((((((t1_0 s0) < t) \<and> ((((b_1 s0) \<and> (A32 s)) \<and> ((t1_0 s) <= (t + 1))) \<or> (((t1_0 s) <= ((t1_0 s0) + 1)) \<and> (A2 s)))) \<or> (((t1_0 s0) >= t) \<and> ((t1_0 s) <= ((t1_0 s0) + 1)))) \<and> ((b_0 s0) \<or> ((\<not> (A12 s)) \<or> (((b_1 s0) \<and> (A32 s)) \<or> (((t1_0 s) = 0) \<and> (A2 s)))))) \<and> ((b_0 s) --> (\<not> (A11 s)))) \<and> ((b_1 s) --> (A31 s))) \<Longrightarrow>
+P4_3_inv_part t b_0 b_1 t1_0 A11 A12 A2 A31 A32 s"
 
 unfolding P4_3_inv_part_def P4_3_part_def
 apply(simp add: P4_3_inv_saving_gen always_imp_refl)
 done
 
 lemma P4_3einv_imp_req: "
-P4_3_inv_part t b_0 b_1 t1_0 A11 A12 A21 A22 A3 s \<Longrightarrow>
+P4_3_inv_part t b_0 b_1 t1_0 A11 A12 A2 A31 A32 s \<Longrightarrow>
 toEnvP s \<Longrightarrow>
 True \<Longrightarrow>
-P4_3_part t A11 A12 A21 A22 A3 s"
+P4_3_part t A11 A12 A2 A31 A32 s"
 
 unfolding P4_3_inv_part_def P4_3_part_def
 apply(simp add: P4_3einv_imp_req_gen always_imp_refl)
@@ -2264,9 +2264,9 @@ done
 
 
 
-lemmas P4_3_used_patterns = P4_3_def always_def weak_previous_def constrained_weak_until_def previous_def 
+lemmas P4_3_used_patterns = P4_3_def always_used_patterns weak_previous_def constrained_weak_until_def previous_def 
 
-lemmas P4_3_inv_used_patterns = P4_3_inv_def always_inv_def weak_previous_def constrained_weak_until_inv_def previous_def previous_inv_def previous_inv_def 
+lemmas P4_3_inv_used_patterns = P4_3_inv_def always_inv_used_patterns weak_previous_def constrained_weak_until_inv_def previous_def previous_inv_def previous_inv_def 
 
 lemmas P4_3_inv_part_used_patterns = P4_3_inv_part_def P4_3_inv_used_patterns
 
@@ -2525,9 +2525,9 @@ done
 
 
 
-lemmas P6_1_used_patterns = P6_1_def always_def weak_previous_def dual_since_def 
+lemmas P6_1_used_patterns = P6_1_def always_used_patterns weak_previous_def dual_since_def 
 
-lemmas P6_1_inv_used_patterns = P6_1_inv_def always_inv_def weak_previous_def dual_since_def previous_inv_def dual_since_def dual_since_inv_def 
+lemmas P6_1_inv_used_patterns = P6_1_inv_def always_inv_used_patterns weak_previous_def dual_since_def previous_inv_def dual_since_def dual_since_inv_def 
 
 lemmas P6_1_inv_part_used_patterns = P6_1_inv_part_def P6_1_inv_used_patterns
 
@@ -2839,9 +2839,9 @@ done
 
 
 
-lemmas P6_2_used_patterns = P6_2_def always_def weak_previous_def dual_since_def weak_until_def 
+lemmas P6_2_used_patterns = P6_2_def always_used_patterns weak_previous_def dual_since_def weak_until_def 
 
-lemmas P6_2_inv_used_patterns = P6_2_inv_def always_inv_def weak_previous_def dual_since_def weak_until_inv_def previous_inv_def dual_since_def dual_since_inv_def 
+lemmas P6_2_inv_used_patterns = P6_2_inv_def always_inv_used_patterns weak_previous_def dual_since_def weak_until_inv_def previous_inv_def dual_since_def dual_since_inv_def 
 
 lemmas P6_2_inv_part_used_patterns = P6_2_inv_part_def P6_2_inv_used_patterns
 
@@ -3109,86 +3109,102 @@ done
 
 
 
-lemmas P_constrained_always_after_max_delay_used_patterns = P_constrained_always_after_max_delay_def P1_2_def constrained_always_def 
+lemmas P_constrained_always_after_max_delay_used_patterns = P_constrained_always_after_max_delay_def P1_2_used_patterns constrained_always_def 
 
-lemmas P_constrained_always_after_max_delay_inv_used_patterns = P_constrained_always_after_max_delay_inv_def P1_2_inv_def constrained_always_inv_def 
+lemmas P_constrained_always_after_max_delay_inv_used_patterns = P_constrained_always_after_max_delay_inv_def P1_2_inv_used_patterns constrained_always_inv_def 
 
 lemmas P_constrained_always_after_max_delay_inv_part_used_patterns = P_constrained_always_after_max_delay_inv_part_def P_constrained_always_after_max_delay_inv_used_patterns
 
 lemmas P_constrained_always_after_max_delay_part_used_patterns = P_constrained_always_after_max_delay_part_def P_constrained_always_after_max_delay_used_patterns
 
-definition P5 where "P5 A11 A12 A2 A3 A4 s \<equiv> (P3_4 A11 A12 (\<lambda> r2 r1 . (\<not> (A2 r1))) (\<lambda> r2 r1 . (((A2 r1) \<and> (A4 r2 r1)) \<or> (A3 r2 r1))) s)"
+definition P5 where "P5 A11 A12 A2 A31 A32 A4 s \<equiv> (P3_4 A11 A12 (\<lambda> r2 r1 . (\<not> (A2 r1))) (\<lambda> r2 r1 . (((A2 r1) \<and> (A4 r2 r1)) \<or> ((previous A31 r2 r1) \<and> (A32 r2 r1)))) s)"
 
-definition P5_part where "P5_part A11 A12 A2 A3 A4 s \<equiv> (P5 A11 A12 A2 (\<lambda> s s1 . (A3 s1)) (\<lambda> s s1 . (A4 s1)) s)"
+definition P5_part where "P5_part A11 A12 A2 A31 A32 A4 s \<equiv> (P5 A11 A12 A2 (\<lambda> s s1 . (A31 s1)) (\<lambda> s s1 . (A32 s1)) (\<lambda> s s1 . (A4 s1)) s)"
 
-definition P5_inv where "P5_inv b_0_0 b_1_0 w_0_0 A11 A12 A2 A3_1 A4_1 s \<equiv> (P3_4_inv b_0_0 b_1_0 w_0_0 A11 A12 (\<lambda> r2 r1 . (\<not> (A2 r1))) (\<lambda> r2 r1 . (((A2 r1) \<and> (A4_1 r2 r1)) \<or> (A3_1 r2 r1))) s)"
+definition P5_inv where "P5_inv b_0 b_0_0 b_1_0 w_0_0 A11 A12 A2 A31_1 A32_1 A4_1 s \<equiv> ((P3_4_inv b_0_0 b_1_0 w_0_0 A11 A12 (\<lambda> r2 r1 . (\<not> (A2 r1))) (\<lambda> r2 r1 . (((A2 r1) \<and> (A4_1 r2 r1)) \<or> ((previous A31_1 r2 r1) \<and> (A32_1 r2 r1)))) s) \<and> (previous_inv b_0 A31_1 s))"
 
-definition P5_inv_part where "P5_inv_part b_0_0 b_1_0 w_0_0 A11 A12 A2 A3 A4 s \<equiv> (P5_inv b_0_0 b_1_0 w_0_0 A11 A12 A2 (\<lambda> s s1 . (A3 s1)) (\<lambda> s s1 . (A4 s1)) s)"
+definition P5_inv_part where "P5_inv_part b_0 b_0_0 b_1_0 w_0_0 A11 A12 A2 A31 A32 A4 s \<equiv> (P5_inv b_0 b_0_0 b_1_0 w_0_0 A11 A12 A2 (\<lambda> s s1 . (A31 s1)) (\<lambda> s s1 . (A32 s1)) (\<lambda> s s1 . (A4 s1)) s)"
 
 lemma P5_inv_saving_gen: "
-P5_inv b_0_0 b_1_0 w_0_0 A11 A12 A2 A3_1 A4_1 s0 \<Longrightarrow>
+P5_inv b_0 b_0_0 b_1_0 w_0_0 A11 A12 A2 A31_1 A32_1 A4_1 s0 \<Longrightarrow>
 consecutive s0 s \<Longrightarrow>
-(((((True \<and> True) \<and> (True \<and> (((True \<and> (always_imp s0 (\<lambda> r1 . (A4_1 s0 r1)) (\<lambda> r1 . (A4_1 s r1)))) \<and> (always_imp s0 (\<lambda> r1 . (A3_1 s0 r1)) (\<lambda> r1 . (A3_1 s r1)))) \<and> ((\<not> (w_0_0 s0)) \<or> ((((A2 s) \<and> (A4_1 s s)) \<or> (A3_1 s s)) \<or> ((w_0_0 s) \<and> (\<not> (A2 s)))))))) \<and> (((b_1_0 s0) \<and> (True \<and> True)) \<or> ((((A2 s) \<and> (A4_1 s s)) \<or> (A3_1 s s)) \<or> ((w_0_0 s) \<and> (\<not> (A2 s)))))) \<and> ((b_1_0 s) --> (((b_0_0 s0) \<and> True) \<or> (\<not> (A12 s))))) \<and> ((b_0_0 s) --> (\<not> (A11 s)))) \<Longrightarrow>
-P5_inv b_0_0 b_1_0 w_0_0 A11 A12 A2 A3_1 A4_1 s"
+((((((True \<and> True) \<and> (True \<and> (((True \<and> (always_imp s0 (\<lambda> r1 . (A4_1 s0 r1)) (\<lambda> r1 . (A4_1 s r1)))) \<and> ((always_imp s0 (A31_1 s0) (A31_1 s)) \<and> (always_imp s0 (\<lambda> r1 . (A32_1 s0 r1)) (\<lambda> r1 . (A32_1 s r1))))) \<and> ((\<not> (w_0_0 s0)) \<or> ((((A2 s) \<and> (A4_1 s s)) \<or> (((b_0 s0) \<and> (always_imp s0 (A31_1 s0) (A31_1 s))) \<and> (A32_1 s s))) \<or> ((w_0_0 s) \<and> (\<not> (A2 s)))))))) \<and> (((b_1_0 s0) \<and> (True \<and> True)) \<or> ((((A2 s) \<and> (A4_1 s s)) \<or> (((b_0 s0) \<and> (always_imp s0 (A31_1 s0) (A31_1 s))) \<and> (A32_1 s s))) \<or> ((w_0_0 s) \<and> (\<not> (A2 s)))))) \<and> ((b_1_0 s) --> (((b_0_0 s0) \<and> True) \<or> (\<not> (A12 s))))) \<and> ((b_0_0 s) --> (\<not> (A11 s)))) \<and> ((b_0 s) --> (A31_1 s s))) \<Longrightarrow>
+P5_inv b_0 b_0_0 b_1_0 w_0_0 A11 A12 A2 A31_1 A32_1 A4_1 s"
 
 unfolding P5_inv_def
+apply(erule conjE)
+apply(erule conjE)
+subgoal premises prems1
+apply(rule conjI)
+apply(insert prems1(1,2,4))[1]
 apply(erule P3_4_inv_saving_gen)
   apply simp
   apply(erule conjE)
-  subgoal premises prems1
+  subgoal premises prems2
   apply(rule conjI)
-  apply(insert prems1(1,2))[1]
+  apply(insert prems2(1,2))[1]
     apply(erule conjE)
-    subgoal premises prems2
+    subgoal premises prems3
     apply(rule conjI)
-    apply(insert prems2(1,2))[1]
+    apply(insert prems3(1,2))[1]
       apply(erule conjE)
-      subgoal premises prems3
+      subgoal premises prems4
       apply(rule conjI)
-      apply(insert prems3(1,2))[1]
+      apply(insert prems4(1,2))[1]
         apply(erule conjE)
-        subgoal premises prems4
+        subgoal premises prems5
         apply(rule conjI)
-        apply(insert prems4(1,2))[1]
-          apply(erule conjE)
-          subgoal premises prems5
-          apply(rule conjI)
-          apply(insert prems5(1,2))[1]
-            apply assumption
-          apply(insert prems5(1,3))
-            apply assumption
-          done
-        apply(insert prems4(1,3))
+        apply(insert prems5(1,2))[1]
           apply(erule conjE)
           subgoal premises prems6
           apply(rule conjI)
           apply(insert prems6(1,2))[1]
-            apply(rule always_imp_refl)
+            apply assumption
           apply(insert prems6(1,3))
+            apply assumption
+          done
+        apply(insert prems5(1,3))
+          apply(erule conjE)
+          subgoal premises prems7
+          apply(rule conjI)
+          apply(insert prems7(1,2))[1]
+            apply(rule always_imp_refl)
+          apply(insert prems7(1,3))
             apply(erule conjE)
-            subgoal premises prems7
+            subgoal premises prems8
             apply(rule conjI)
-            apply(insert prems7(1,2))[1]
+            apply(insert prems8(1,2))[1]
               apply(rule always_disj_rule)
               apply simp
                 apply(erule conjE)
-                subgoal premises prems8
+                subgoal premises prems9
                 apply(rule conjI)
-                apply(insert prems8(1,2))[1]
+                apply(insert prems9(1,2))[1]
                   apply(rule always_conj_rule)
                   apply simp
                     apply(erule conjE)
-                    subgoal premises prems9
+                    subgoal premises prems10
                     apply(rule conjI)
-                    apply(insert prems9(1,2))[1]
+                    apply(insert prems10(1,2))[1]
                       apply(rule always_imp_refl)
-                    apply(insert prems9(1,3))
+                    apply(insert prems10(1,3))
                       apply assumption
                     done
-                apply(insert prems8(1,3))
-                  apply assumption
+                apply(insert prems9(1,3))
+                  apply(rule always_conj_rule)
+                  apply simp
+                    apply(erule conjE)
+                    subgoal premises prems11
+                    apply(rule conjI)
+                    apply(insert prems11(1,2))[1]
+                      apply(rule previous_LS4)
+                      apply simp
+                        apply assumption
+                    apply(insert prems11(1,3))
+                      apply assumption
+                    done
                 done
-            apply(insert prems7(1,3))
+            apply(insert prems8(1,3))
               apply(erule disjE)
               apply(rule disjI1)
                 apply assumption
@@ -3198,42 +3214,58 @@ apply(erule P3_4_inv_saving_gen)
                   apply(erule disjE)
                   apply(rule disjI1)
                     apply(erule conjE)
-                    subgoal premises prems10
+                    subgoal premises prems12
                     apply(rule conjI)
-                    apply(insert prems10(1,2))[1]
+                    apply(insert prems12(1,2))[1]
                       apply assumption
-                    apply(insert prems10(1,3))
+                    apply(insert prems12(1,3))
                       apply assumption
                     done
                   apply(rule disjI2)
-                    apply assumption
+                    apply(erule conjE)
+                    subgoal premises prems13
+                    apply(rule conjI)
+                    apply(insert prems13(1,2))[1]
+                      apply(rule previous_one_point[OF prems1(3)])
+                      apply simp
+                        apply(erule conjE)
+                        subgoal premises prems14
+                        apply(rule conjI)
+                        apply(insert prems14(1,2))[1]
+                          apply assumption
+                        apply(insert prems14(1,3))
+                          apply assumption
+                        done
+                    apply(insert prems13(1,3))
+                      apply assumption
+                    done
                 apply(rule disjI2)
                   apply(erule conjE)
-                  subgoal premises prems11
+                  subgoal premises prems15
                   apply(rule conjI)
-                  apply(insert prems11(1,2))[1]
+                  apply(insert prems15(1,2))[1]
                     apply assumption
-                  apply(insert prems11(1,3))
+                  apply(insert prems15(1,3))
                     apply assumption
                   done
             done
           done
         done
-      apply(insert prems3(1,3))
+      apply(insert prems4(1,3))
         apply(erule disjE)
         apply(rule disjI1)
           apply(erule conjE)
-          subgoal premises prems12
+          subgoal premises prems16
           apply(rule conjI)
-          apply(insert prems12(1,2))[1]
+          apply(insert prems16(1,2))[1]
             apply assumption
-          apply(insert prems12(1,3))
+          apply(insert prems16(1,3))
             apply(erule conjE)
-            subgoal premises prems13
+            subgoal premises prems17
             apply(rule conjI)
-            apply(insert prems13(1,2))[1]
+            apply(insert prems17(1,2))[1]
               apply assumption
-            apply(insert prems13(1,3))
+            apply(insert prems17(1,3))
               apply assumption
             done
           done
@@ -3243,63 +3275,95 @@ apply(erule P3_4_inv_saving_gen)
             apply(erule disjE)
             apply(rule disjI1)
               apply(erule conjE)
-              subgoal premises prems14
+              subgoal premises prems18
               apply(rule conjI)
-              apply(insert prems14(1,2))[1]
+              apply(insert prems18(1,2))[1]
                 apply assumption
-              apply(insert prems14(1,3))
+              apply(insert prems18(1,3))
                 apply assumption
               done
             apply(rule disjI2)
-              apply assumption
+              apply(erule conjE)
+              subgoal premises prems19
+              apply(rule conjI)
+              apply(insert prems19(1,2))[1]
+                apply(rule previous_one_point[OF prems1(3)])
+                apply simp
+                  apply(erule conjE)
+                  subgoal premises prems20
+                  apply(rule conjI)
+                  apply(insert prems20(1,2))[1]
+                    apply assumption
+                  apply(insert prems20(1,3))
+                    apply assumption
+                  done
+              apply(insert prems19(1,3))
+                apply assumption
+              done
           apply(rule disjI2)
             apply(erule conjE)
-            subgoal premises prems15
+            subgoal premises prems21
             apply(rule conjI)
-            apply(insert prems15(1,2))[1]
+            apply(insert prems21(1,2))[1]
               apply assumption
-            apply(insert prems15(1,3))
+            apply(insert prems21(1,3))
               apply assumption
             done
       done
-    apply(insert prems2(1,3))
+    apply(insert prems3(1,3))
       apply(rule impI)
       apply(erule impE)
       apply assumption
-      subgoal premises prems16
-      apply(insert prems16(1,3))
+      subgoal premises prems22
+      apply(insert prems22(1,3))
         apply(erule disjE)
         apply(rule disjI1)
           apply(erule conjE)
-          subgoal premises prems17
+          subgoal premises prems23
           apply(rule conjI)
-          apply(insert prems17(1,2))[1]
+          apply(insert prems23(1,2))[1]
             apply assumption
-          apply(insert prems17(1,3))
+          apply(insert prems23(1,3))
             apply assumption
           done
         apply(rule disjI2)
           apply assumption
       done
     done
-  apply(insert prems1(1,3))
+  apply(insert prems2(1,3))
     apply(rule impI)
     apply(erule impE)
     apply assumption
-    subgoal premises prems18
-    apply(insert prems18(1,3))
+    subgoal premises prems24
+    apply(insert prems24(1,3))
       apply assumption
     done
   done
+apply(insert prems1(1,3,5))
+  apply(erule previous_rule)
+  apply simp
+  apply(rule impI)
+  apply(erule impE)
+  apply assumption
+  subgoal premises prems25
+  apply(insert prems25(1,3))
+    apply assumption
+  done
+done
 done
 
 lemma P5einv_imp_req_gen: "
-P5_inv b_0_0 b_1_0 w_0_0 A11 A12 A2 A3_1 A4_1 s0 \<Longrightarrow>
+P5_inv b_0 b_0_0 b_1_0 w_0_0 A11 A12 A2 A31_1 A32_1 A4_1 s0 \<Longrightarrow>
 toEnvP s0 \<Longrightarrow>
-((True \<and> True) \<and> (True \<and> ((True \<and> (always_imp s0 (\<lambda> r1 . (A4_1 s0 r1)) (\<lambda> r1 . (A4 s0 r1)))) \<and> (always_imp s0 (\<lambda> r1 . (A3_1 s0 r1)) (\<lambda> r1 . (A3 s0 r1)))))) \<Longrightarrow>
-P5 A11 A12 A2 A3 A4 s0"
+((True \<and> True) \<and> (True \<and> ((True \<and> (always_imp s0 (\<lambda> r1 . (A4_1 s0 r1)) (\<lambda> r1 . (A4 s0 r1)))) \<and> ((always_imp s0 (A31_1 s0) (A31 s0)) \<and> (always_imp s0 (\<lambda> r1 . (A32_1 s0 r1)) (\<lambda> r1 . (A32 s0 r1))))))) \<Longrightarrow>
+P5 A11 A12 A2 A31 A32 A4 s0"
 
 unfolding P5_inv_def P5_def
+subgoal premises prems1
+apply(insert prems1(1,2))
+apply(erule conjE)
+subgoal premises prems2
+apply(insert prems2(1,2) prems1(3))
 apply(erule P3_4einv_imp_req_gen)
 apply simp
   apply(erule conjE)
@@ -3338,27 +3402,40 @@ apply simp
               apply assumption
             done
         apply(insert prems6(1,3))
-          apply assumption
+          apply(rule always_conj_rule)
+          apply simp
+            apply(erule conjE)
+            subgoal premises prems8
+            apply(rule conjI)
+            apply(insert prems8(1,2))[1]
+              apply(rule previous_LS5)
+              apply simp
+                apply assumption
+            apply(insert prems8(1,3))
+              apply assumption
+            done
         done
     done
   done
 done
+done
+done
 
 lemma P5_inv_saving: "
-P5_inv_part b_0_0 b_1_0 w_0_0 A11 A12 A2 A3 A4 s0 \<Longrightarrow>
+P5_inv_part b_0 b_0_0 b_1_0 w_0_0 A11 A12 A2 A31 A32 A4 s0 \<Longrightarrow>
 consecutive s0 s \<Longrightarrow>
-(((((\<not> (w_0_0 s0)) \<or> ((((A2 s) \<and> (A4 s)) \<or> (A3 s)) \<or> ((w_0_0 s) \<and> (\<not> (A2 s))))) \<and> ((b_1_0 s0) \<or> ((((A2 s) \<and> (A4 s)) \<or> (A3 s)) \<or> ((w_0_0 s) \<and> (\<not> (A2 s)))))) \<and> ((b_1_0 s) --> ((b_0_0 s0) \<or> (\<not> (A12 s))))) \<and> ((b_0_0 s) --> (\<not> (A11 s)))) \<Longrightarrow>
-P5_inv_part b_0_0 b_1_0 w_0_0 A11 A12 A2 A3 A4 s"
+((((((\<not> (w_0_0 s0)) \<or> ((((A2 s) \<and> (A4 s)) \<or> ((b_0 s0) \<and> (A32 s))) \<or> ((w_0_0 s) \<and> (\<not> (A2 s))))) \<and> ((b_1_0 s0) \<or> ((((A2 s) \<and> (A4 s)) \<or> ((b_0 s0) \<and> (A32 s))) \<or> ((w_0_0 s) \<and> (\<not> (A2 s)))))) \<and> ((b_1_0 s) --> ((b_0_0 s0) \<or> (\<not> (A12 s))))) \<and> ((b_0_0 s) --> (\<not> (A11 s)))) \<and> ((b_0 s) --> (A31 s))) \<Longrightarrow>
+P5_inv_part b_0 b_0_0 b_1_0 w_0_0 A11 A12 A2 A31 A32 A4 s"
 
 unfolding P5_inv_part_def P5_part_def
 apply(simp add: P5_inv_saving_gen always_imp_refl)
 done
 
 lemma P5einv_imp_req: "
-P5_inv_part b_0_0 b_1_0 w_0_0 A11 A12 A2 A3 A4 s \<Longrightarrow>
+P5_inv_part b_0 b_0_0 b_1_0 w_0_0 A11 A12 A2 A31 A32 A4 s \<Longrightarrow>
 toEnvP s \<Longrightarrow>
 True \<Longrightarrow>
-P5_part A11 A12 A2 A3 A4 s"
+P5_part A11 A12 A2 A31 A32 A4 s"
 
 unfolding P5_inv_part_def P5_part_def
 apply(simp add: P5einv_imp_req_gen always_imp_refl)
@@ -3366,9 +3443,9 @@ done
 
 
 
-lemmas P5_used_patterns = P5_def P3_4_def 
+lemmas P5_used_patterns = P5_def P3_4_used_patterns previous_def 
 
-lemmas P5_inv_used_patterns = P5_inv_def P3_4_inv_def 
+lemmas P5_inv_used_patterns = P5_inv_def P3_4_inv_used_patterns previous_def previous_inv_def 
 
 lemmas P5_inv_part_used_patterns = P5_inv_part_def P5_inv_used_patterns
 
